new type definitions

project/csp_syntax.v
@@ -1,69 +1,114 @@
 Require Import Coq.Lists.ListSet.
 Require Import Coq.Lists.List.
-Import ListNotations.
+Require Import Coq.Setoids.Setoid.
+Require Import Coq.Strings.String.
+
 Module CSP_Syntax.
 
-(* Define Event type *)
-Definition Event: Type := nat.
+Set Implicit Arguments.
+Import ListNotations.
+Open Scope string_scope.
+
+Definition Event: Type := string.
 
 Theorem Event_eq_dec: forall (x y: Event), {x = y} + {x <> y}.
 Proof.
-Admitted.
+  apply string_dec.
+Qed.
 
-(* A set of events should be in context? *)
+Definition Alphabet: Type := set Event.
 
 Inductive Proc: Type :=
   | Stop: Proc
+  | Skip: Proc
   | ProcPref: Event -> Proc -> Proc
   | ProcExtChoice: Proc -> Proc -> Proc
   | ProcCond: bool -> Proc -> Proc -> Proc
-  | ProcRec: Proc -> Proc. 
+  | ProcName: string -> Proc. 
   
-Notation "a --> p" := (ProcPref a p)
+Inductive DefProc: Type :=
+  | Def: string -> Proc -> DefProc.
+
+Inductive Spec: Type :=
+  | SpecDef: Alphabet -> list DefProc -> Spec. 
+
+Module CSP_Syntax_Notations.
+(* set notations *)
+
+(*TODO: Think about using list instead of set for convenience *)
+(*
+Notation "{ }" := nil (format "{ }").
+Notation "{ x }" := (set_add _ x nil).
+Notation "{ x ; y ; .. ; z }" := (set_add _ x (set_add _ y .. (set_add _ z nil) ..)).
+*)
+
+(* CSP *)
+Notation "a -->> p" := (ProcPref a p)
   (at level 60, right associativity).
                       
-Notation "p [] q" := (ProcExtChoice p q)
+Notation "p [-] q" := (ProcExtChoice p q)
   (at level 60, right associativity).
                      
 Notation "'if' b 'then' p 'else' q" := (ProcCond b p q)
   (at level 60, right associativity).
 
+Notation "p '" := (ProcName p)
+  (at level 60, no associativity).
+
+Notation "p ::= q" := (Def p q)
+  (at level 99, no associativity).
+
+Notation "'channel' a , 'definitions' ds" := (SpecDef a ds)
+  (at level 99, no associativity).
+  
+Check "P"'.
+(* Notation for lists that are sets using set_add *)
+
+Example procTest := channel ["a"; "b"],
+  definitions ["P" ::= ("a" -->> Stop) [-] ("b" -->> Stop)].
+
+Check procTest.
+
+End CSP_Syntax_Notations.
+
+Import CSP_Syntax_Notations.
+
+Fixpoint process_names (spec: Spec): list string :=
+  match spec with (SpecDef a procs) =>
+    map (fun d => match d with (Def s _) => s end) procs
+  end.
+
+Compute process_names procTest.
+
+Search "distinct".
+Search "unique".
+
+Fixpoint distinct {T: Type}
+  (T_eq_dec: forall (x y: T), {x = y} + {x <> y}) (l: list T): Prop :=
+  match l with
+  | [] => True
+  | t :: l' => let t_unique := In t l' in
+    t_unique /\ distinct T_eq_dec l'
+  end.
+
 Definition Trace: Type := list Event.
 
 Theorem Trace_eq_dec: forall (x y: Trace), {x = y} + {x <> y}.
 Proof.
-(* Utilizar prova de que se há uma igualdade para os elementos da lista, então pode-se
-  definir uma igualdade para a lista
-*)
-Admitted.
+  Search "list_eq_dec". apply list_eq_dec. apply Event_eq_dec.
+Qed.
+
+(* Trace and set of Traces definitions *)
 
 Definition emptyTrace: Trace := nil.
 
-Check set_add.
-
 Definition setAdd := set_add Trace_eq_dec.
-
-Check setAdd.
 
 Definition sngTrace (e: Trace) := setAdd e (empty_set _).
 
 Definition setUnion := set_union Trace_eq_dec.
 
-Definition sngEmptyTrace := sngTrace emptyTrace.
-
 Definition setMap := @set_map Trace Trace Trace_eq_dec.
-
-Fixpoint traces (p: Proc): set Trace :=
-  match p with
-  | Stop => [emptyTrace]
-  | ProcPref e q =>
-    let qTraces := traces(q) in
-    let qWithA := setMap (fun trace => e :: trace) qTraces in
-      setUnion [emptyTrace] qWithA
-  | ProcExtChoice p q => setUnion (traces p) (traces q)
-  | ProcCond b p q => if b then (traces p) else (traces q)
-  | _ => [emptyTrace]
-  end.    
 
 Lemma set_union_not_empty: forall {T: Type}
   {T_eq_dec: forall (x y: T), {x = y} + {x <> y}}
@@ -83,10 +128,25 @@ Proof.
   unfold empty_set. intros H. inversion H.
 Qed.
 
+(* Functional definition of the set of traces of a process*)
+Fixpoint traces (p: Proc): set Trace :=
+  match p with
+  | Stop => [[]]
+  | Skip => [[]]
+  | ProcPref e q =>
+    let qTraces := traces(q) in
+    let qWithA := setMap (fun trace => e :: trace) qTraces in
+      setUnion [[]] qWithA
+  | ProcExtChoice p q => setUnion (traces p) (traces q)
+  | ProcCond b p q => if b then (traces p) else (traces q)
+  | _ => [[]]
+  end.    
+
 Theorem traces_non_empty: forall (p: Proc),
   traces p <> empty_set Trace.
 Proof.
   intros p. induction p.
+  - simpl. unfold empty_set. intros H. inversion H.
   - simpl. unfold empty_set. intros H. inversion H.
   - simpl. unfold setUnion. simpl. Search (_ <> empty_set).
     apply set_union_not_empty. apply sngTrace_not_empty.
@@ -97,6 +157,7 @@ Proof.
   - simpl. apply sngTrace_not_empty. 
 Qed.
 
+(* Maybe write Prop definition of what it means to be a prefix of a list *)
 Fixpoint prefixes {T: Type} (s: list T): list (list T) :=
   match s with
   | nil => [nil]
@@ -105,12 +166,44 @@ Fixpoint prefixes {T: Type} (s: list T): list (list T) :=
     nil :: map (fun p => a :: p) ps'
   end.
 
-(*
-Definir prop prefixClosed e provar teorema abaixo.
+Definition prefix_closed {T: Type} (tSet: set (list T)): Prop :=
+  forall (tList: list T),
+    In tList tSet ->
+    forall (prefT: list T),
+      In prefT (prefixes tList) ->
+        In prefT tSet.
+
+Check prefix_closed.
+
+Theorem or_false: forall (P: Prop), P \/ False <-> P.
+Proof.
+  intros P.
+  split.
+  - intros. inversion H.
+    + apply H0.
+    + inversion H0.
+  - intros HP. left. apply HP. 
+Qed.
 
 Theorem traces_prefix_closed: forall (p: Proc),
-  prefixClosed (traces p).
-*)
+  prefix_closed (traces p).
+Proof.
+  intros p. induction p.
+  - simpl. unfold prefix_closed.
+    intros. simpl in H. rewrite -> or_false in H.
+    subst tList. simpl in H0. rewrite -> or_false in H0.
+    subst prefT. unfold emptyTrace. simpl. left. reflexivity.
+  - simpl. unfold prefix_closed.
+    intros. simpl in H. rewrite -> or_false in H.
+    subst tList. simpl in H0. rewrite -> or_false in H0.
+    subst prefT. unfold emptyTrace. simpl. left. reflexivity.
+  - simpl. unfold prefix_closed. intros.
+    unfold prefix_closed in IHp. apply set_union_intro.
+    destruct tList.
+    + simpl in H0. rewrite or_false in H0. left. rewrite <- H0.
+      unfold emptyTrace. simpl. left. reflexivity.
+    + simpl in H0.
+Abort.
   
   
 
